examples/bug-reports/bug189.fst
@@ -1,0 +1,16 @@
+module Bug189
+
+type heap = unit -> Tot unit
+
+type pred = heap -> Tot unit
+
+type deduce : unit -> Type =
+| Blah : deduce ()
+
+val feq : #a:Type -> a -> Tot unit
+let feq x = ()
+
+type hoare_c (q:pred) = (h':heap -> deduce (q h'))
+
+val skip_spec : u:unit -> Tot (hoare_c feq)
+let skip_spec u = fun h1 -> magic()
